Lib/Derivation.v
@@ -30,23 +30,21 @@ with derivesForest {g : grammar} :
                        (prefix ++ suffix) 
                        (Fcons hdTree tlTrees).
 
-Definition derivesMaximalTree (g : grammar)
+Definition symDerivesMaximalPrefix (g : grammar)
            (sym : symbol) (pre suf : list string)
            (tree : tree) :=
     (@derivesTree g) sym pre tree
     /\ forall pre' suf' tree',
       (pre ++ suf)%list = (pre' ++ suf')%list
         -> (@derivesTree g) sym pre' tree'
-        -> span tree' <= span tree.
+        -> List.length pre' <= List.length pre.
 
-Definition derivesMaximalForest (g : grammar)
-           (x : nonterminal) (gamma : list symbol)
+Definition gammaDerivesMaximalPrefix (g : grammar)
+           (gamma : list symbol)
            (pre suf : list string)
            (f : forest) :=
-  In (x, gamma) (productions g)
-  /\ (@derivesForest g) gamma pre f
-  /\ forall gamma' pre' suf' f',
-      In (x, gamma') (productions g)
-      -> (pre ++ suf)%list = (pre' ++ suf')%list
-      -> (@derivesForest g) gamma' pre' f'
-      -> spanForest f' <= spanForest f.
+  (@derivesForest g) gamma pre f
+  /\ forall pre' suf' f',
+      (pre ++ suf)%list = (pre' ++ suf')%list
+      -> (@derivesForest g) gamma pre' f'
+      -> List.length pre' <= List.length pre.
