LL1/CompletenessProof.v
@@ -2,6 +2,7 @@ Require Import List Omega String.
 Require Import Derivation Grammar Lemmas ParseTable
         ParseTree LL1.Parser Lib.Tactics
         LL1.CorrectnessProof LL1.MonotonicityLemmas.
+Open Scope string_scope.
 
 Conjecture in_grammar_lookup :
   forall tbl g x gamma,
@@ -124,87 +125,6 @@ Conjecture lookup_parseForest :
        (Some f, suffix)
     -> parseTableLookup x (peek input) tbl = Some gamma.
 
-Lemma at_most_one_sym_succeeds :
-  forall tbl g,
-    isParseTableFor tbl g
-    -> forall tr x input fuel suffix,
-      parse tbl (NT x) input fuel = (Some tr, suffix)
-      -> forall x' tr' suffix',
-        x <> x'
-        -> ~parse tbl (NT x') input fuel =
-           (Some tr', suffix').
-Proof.
-  intros tbl g Htbl.
-    induction tr as [ s
-                  | s f IHparseForest
-                  |
-                  | tr IHparse f IHparseForest ]
-      using tree_mutual_ind with
-        (P := fun tr =>
-                forall x input fuel suffix,
-                  parse tbl (NT x) input fuel =
-                  (Some tr, suffix)
-                -> forall x' tr' suffix',
-                  x <> x'
-                  -> ~parse tbl (NT x') input fuel =
-                     (Some tr', suffix'))
-        
-        (P0 := fun subtrees =>
-                 forall gamma input fuel suffix,
-                   parseForest tbl gamma input fuel =
-                   (Some subtrees, suffix)
-                   -> forall gamma' subtrees' suffix',
-                     gamma <> gamma'
-                     -> ~parseForest tbl gamma' input fuel =
-                        (Some subtrees', suffix)).
-
-
-  - unfold not; intros.
-    apply H0.
-    destruct fuel; sim.
-    + inv H.
-    + destruct (parseTableLookup x (peek input) tbl)
-        as [gamma |] eqn:Hlkp;
-        destruct (parseTableLookup x' (peek input) tbl)
-        as [gamma' |] eqn:Hlkp'.
-      * destruct (parseForest tbl gamma input fuel)
-          as (o, input') eqn:Hpf.
-        destruct (parseForest tbl gamma' input fuel)
-          as (o', input'').
-        destruct o; destruct o'.
-        { inv H. }
-        { inv H. }
-        { inv H. }
-        { inv H. }
-      * inv H1.
-      * inv H.
-      * inv H.
-
-  - unfold not; intros.
-    destruct fuel; sim.
-    + inv H.
-    + destruct (parseTableLookup x (peek input) tbl)
-        as [gamma |] eqn:Hlkp;
-      destruct (parseTableLookup x' (peek input) tbl)
-        as [gamma' |] eqn:Hlkp'.
-      * destruct (parseForest tbl gamma input fuel)
-          as (o, input') eqn:Hpf.
-        destruct (parseForest tbl gamma' input fuel)
-          as (o', input'') eqn:Hpf'.
-        destruct o; destruct o'.
-        { inv H.
-          inv H1.
-          eapply IHparseForest.
-          { eapply Hpf. }
-          { eauto. }
-          { unfold not; intros.
-            apply H0.
-            rewrite <- H in Hpf'.
-            rewrite Hpf in Hpf'.
-            inv Hpf'.
-            rewrite <- Hlkp in Hlkp'.
-Abort. (* seems promising, though *)
-
 
 Lemma derivesTree_lookup :
   forall g x prefix f,
@@ -233,51 +153,6 @@ Proof.
   exists gamma; split; trivial.
 Qed.
 
-Lemma der_lookup :
-  forall tbl g,
-    isParseTableFor tbl g
-    -> forall trees x input gamma,
-      (@derivesTree g) (NT x) input (Node x trees)
-      -> (@derivesForest g) gamma input trees
-      -> parseTableLookup x (peek input) tbl = Some gamma.
-Proof.
-  intros tbl g Htbl trees.
-  unfold isParseTableFor in Htbl.
-  destruct Htbl as [Hcom Hmin].
-  destruct Hcom as [Hcomfi Hcomfo].
-  unfold ptCompleteFirst in Hcomfi.
-  unfold ptCompleteFollow in Hcomfo.
-  induction trees as [| tr trs]; intros.
-  - inv H.
-    inv H0.
-    inv H5.
-    simpl in *.
-
-Lemma dd :
-  forall trees g gamma prefix suffix x tbl,
-    (@derivesForest g) gamma prefix trees
-    -> (@derivesTree g) (NT x) prefix (Node x trees)
-    -> isParseTableFor tbl g
-    -> parseTableLookup x (peek (app prefix suffix)) tbl =
-       Some gamma.
-Proof.
-  induction trees as [| st sts]; intros.
-  - inv H.
-    inv H0.
-    inv H5.
-    simpl.
-    unfold isParseTableFor in H1.
-    destruct H1 as [Hcom Hmin].
-    unfold parseTableComplete in Hcom.
-    destruct Hcom as [Hcomfi Hcomfo].
-    unfold ptCompleteFollow in Hcomfo.
-    
-    apply Hcomfo with (y := EOF) in H3.
-    + destruct H3 as [tMap [H3 H4]].
-      unfold parseTableLookup.
-      rewrite H3.
-      trivial.
-Admitted.
 
 Lemma in_grammar_lookup_tbl :
   forall tbl g,
@@ -306,80 +181,331 @@ Proof.
     
   induction gamma as [| sym syms]; intros.
 Abort.
-  
-        
-Conjecture in_grammar_lookup_tbl :
+
+Lemma lookup_exists :
+  forall x la tbl gamma,
+    parseTableLookup x la tbl = Some gamma
+    -> exists laMap,
+      StringMap.find x tbl = Some laMap
+      /\ LookaheadMap.find la laMap = Some gamma.
+Proof.
+  intros.
+  unfold parseTableLookup in H.
+  destruct (StringMap.find x tbl) as [laMap |] eqn:Hsf.
+  - exists laMap; split; trivial.
+  - inv H.
+Qed.
+
+
+Lemma eof_fprod :
+  forall g la x gamma,
+    (@firstProd g) la x gamma
+    -> la = EOF
+    -> False.
+Proof.
+  intros g la x gamma H.
+  induction H using firstProd_mutual_ind with
+      (P := fun la x gamma (pf : firstProd la x gamma) =>
+              la = EOF -> False)
+      (P0 := fun la gamma (pf : firstGamma la gamma) =>
+               la = EOF -> False)
+      (P1 := fun la sym (pf : firstSym la sym) =>
+               la = EOF -> False); intros.
+  - apply IHfirstProd; trivial.
+  - apply IHfirstProd; trivial.
+  - apply IHfirstProd; trivial. 
+  - inv H.
+  - apply IHfirstProd; trivial.
+Qed.
+
+Import ListNotations.
+Theorem parseForest_correct :
+  forall (g   : grammar)
+         (tbl : parse_table),
+    ParseTable.isParseTableFor tbl g ->
+    forall f input gamma suffix fuel,
+      parseForest tbl gamma input fuel =
+      (Some f, suffix) ->
+      exists prefix,
+        (prefix ++ suffix)%list = input /\
+        (@derivesForest g) gamma prefix f.
+Proof.
+  intros g tbl Htbl f.
+  induction f using forest_mutual_ind with
+      (P0 := fun subtrees =>
+               forall input gamma suffix fuel,
+                 parseForest tbl gamma input fuel =
+                 (Some subtrees, suffix) ->
+                 exists prefix,
+                   (prefix ++ suffix)%list = input /\
+                   (@derivesForest g) gamma prefix subtrees)
+      (P := fun tr =>
+              forall input sym suffix fuel,
+                parse tbl sym input fuel = (Some tr, suffix) ->
+                exists prefix,
+                  (prefix ++ suffix)%list = input /\
+                  (@derivesTree g) sym prefix tr).
+
+  - intros input sym suffix fuel Hparse. 
+    destruct fuel as [| fuel].
+    + inv Hparse.
+    + destruct sym as [y | x].
+      * destruct input as [| token input].
+        { inv Hparse. }
+        simpl in Hparse.
+        destruct (Utils.beqString y token) eqn:Hbeq.
+        { inv Hparse. exists [token]. split.
+          { reflexivity. }
+          apply beqString_eq in Hbeq. subst.
+          apply derivesT. }
+        inv Hparse.
+      * apply nt_derives_Node in Hparse. inv Hparse.
+
+  - intros input sym suffix fuel Hparse.
+    destruct fuel as [| fuel].
+    + inv Hparse.
+    + destruct sym as [y | x].
+      * apply t_derives_Leaf in Hparse. inv Hparse.
+      * simpl in Hparse. 
+        destruct (parseTableLookup x (peek input) tbl)
+                 as [ys |] eqn:Hlookup.
+        { destruct (parseForest tbl ys input fuel)
+                   as [subresult input'] eqn:Hforest.
+          { destruct subresult as [subtrees |].
+            { inv Hparse.
+              apply IHf in Hforest.
+              destruct Hforest as [prefix Hforest].
+              exists prefix.
+              destruct Hforest as [Happ Hderives]. split.
+              { assumption. }
+              inv Hderives.
+              { apply derivesNT with (gamma := nil).
+                { simpl in Hlookup. 
+                  apply lookup_tbl_in_grammar with
+                      (g := g)
+                      (x := s)
+                      (y := peek suffix)
+                      (gamma:=nil) in Hlookup.
+                  { assumption. }
+                  assumption. }
+                apply derivesFnil. }
+              apply derivesNT with
+                  (gamma := (hdRoot :: tlRoots)).
+              { eapply lookup_tbl_in_grammar; eassumption. }
+              { apply derivesFcons; assumption. }}
+            { inv Hparse. }}}
+        { inv Hparse. }
+
+  - intros input gamma suffix fuel HparseForest.
+    destruct fuel as [| fuel].
+    + inv HparseForest.
+    + destruct gamma as [| sym gamma'].
+      * simpl in HparseForest. inv HparseForest.
+        exists nil. split.
+        { reflexivity. }
+        apply derivesFnil.
+      * exfalso.
+        simpl in HparseForest.
+        destruct (parse tbl sym input fuel)
+          as [subresult input'].
+        destruct subresult as [lSib |].
+        { destruct (parseForest tbl gamma' input' fuel)
+            as [subresult input''].
+          destruct subresult as [rSibs |].
+          { inv HparseForest. }
+          inv HparseForest. }
+        inv HparseForest.
+
+  - intros input gamma suffix fuel HparseForest.
+    destruct fuel as [| fuel].
+    + inv HparseForest.
+    + destruct gamma as [| sym gamma'].
+      * inv HparseForest.
+      * simpl in HparseForest.
+        destruct (parse tbl sym input fuel)
+          as [subresult input'] eqn:Htree.
+        destruct subresult.
+        { destruct (parseForest tbl gamma' input' fuel)
+            as [subresult input''] eqn:Hforest.
+          destruct subresult as [rSibs |].
+          { inv HparseForest.
+            apply IHf in Htree.
+            { destruct Htree as [treePrefix Htree].
+              destruct Htree as [HappTree HderivesTree].
+              apply IHf0 in Hforest.
+              destruct Hforest as [forestPrefix Hforest].
+              destruct Hforest as [HappForest HderivesForest].
+              subst.
+              exists (treePrefix ++ forestPrefix)%list. split.
+              { rewrite app_assoc. reflexivity. }
+              apply derivesFcons.
+              { assumption. }
+              assumption. }}
+          inv HparseForest. }
+        inv HparseForest.
+Qed.
+
+Lemma derivesForest_nil_nullable :
+  forall f g gamma,
+    (@derivesForest g) gamma [] f
+    -> (@nullableGamma g) gamma.
+Proof.
+  induction f using forest_mutual_ind with
+      (P := fun tr =>
+              forall g x,
+                (@derivesTree g) (NT x) nil tr
+                -> (@nullableSym g) (NT x))
+      (P0 := fun f =>
+               forall g gamma,
+                 (@derivesForest g) gamma nil f
+                 -> (@nullableGamma g) gamma); intros.
+
+  - inv H.
+  - inv H.
+    apply IHf in H5.
+    econstructor.
+    econstructor; eauto.
+  - inv H.
+    constructor.
+  - destruct gamma.
+    + constructor.
+    + inv H.
+      assert (prefix = nil) by
+          (destruct prefix; try inv H2; auto).
+      assert (suffix = nil) by
+          (destruct prefix; try inv H2; auto).
+      subst.
+      inv H4.
+      constructor.
+      * apply IHf.
+        econstructor; eauto.
+      * apply IHf0.
+        auto.
+Qed.
+
+Lemma derivesTree_nil_nullable :
+  forall t g x,
+    (@derivesTree g) (NT x) [] t
+    -> (@nullableSym g) (NT x).
+Proof.
+  induction t using tree_mutual_ind with
+      (P := fun tr =>
+              forall g x,
+                (@derivesTree g) (NT x) nil tr
+                -> (@nullableSym g) (NT x))
+      (P0 := fun f =>
+               forall g gamma,
+                 (@derivesForest g) gamma nil f
+                 -> (@nullableGamma g) gamma); intros.
+
+    - inv H.
+  - inv H.
+    apply IHt in H5.
+    econstructor.
+    econstructor; eauto.
+  - inv H.
+    constructor.
+  - destruct gamma.
+    + constructor.
+    + inv H.
+      assert (prefix = nil) by
+          (destruct prefix; try inv H2; auto).
+      assert (suffix = nil) by
+          (destruct prefix; try inv H2; auto).
+      subst.
+      inv H4.
+      constructor.
+      * apply IHt.
+        econstructor; eauto.
+      * apply IHt0.
+        auto.
+Qed.
+    
+
+Lemma firstProd_not_nil :
   forall tbl g,
     isParseTableFor tbl g
-    -> forall x gamma prefix suffix fuel f,
-      In (x, gamma) (productions g)
-      -> parseForest tbl gamma (app prefix suffix) fuel =
-         (Some f, suffix)
-      -> parseTableLookup x (peek (app prefix suffix)) tbl =
-         Some gamma.
-
-(*
-Theorem parse_complete :
-  forall (g   : grammar)
-         (tbl : parse_table),
-    isParseTableFor tbl g ->
-    forall (tr     : tree)
-           (input  : list string)
-           (sym    : symbol)
-           (prefix suffix : list string),
-      input = (prefix ++ suffix)%list ->
-      (@derivesTree g) sym prefix tr ->
-      match tr with
-      | (Leaf y) => exists fuel,
-                    parse tbl sym input fuel = (Some tr, suffix)
-      | (Node x f) => exists fuel fuel2 gamma,
-                      parseTableLookup x (peek input) tbl = Some gamma
-                      /\ parseForest tbl gamma input fuel = (Some f, suffix)
-                      /\ parse tbl sym input fuel2 = (Some tr, suffix)
-      end.
+    -> forall f x gamma word tok,
+      (@derivesForest g) gamma word f
+      -> (@firstProd g) (LA tok) x gamma
+      -> exists tl,
+          word = tok :: tl.
 Proof.
-  intros g tbl Htbl tr.
-  induction tr as [ s
-                  | s f IHparseForest
-                  |
-                  | tr IHparse f IHparseForest ]
-      using tree_mutual_ind with
+Admitted.
+
+Lemma derivesForest_cons_firstGamma :
+  forall f g tok toks gamma,
+    (@derivesForest g) gamma (tok :: toks) f
+    -> (@firstGamma g) (LA tok) gamma.
+Proof.
+  intro f.
+  induction f using forest_mutual_ind with
+      (P0 := fun f =>
+              forall g tok toks gamma,
+                (@derivesForest g) gamma (tok :: toks) f
+                -> (@firstGamma g) (LA tok) gamma)
       (P := fun tr =>
-              forall input sym prefix suffix,
-              input = (prefix ++ suffix)%list ->
-              (@derivesTree g) sym prefix tr ->
-              match tr with
-              | (Leaf y) => exists fuel,
-                            parse tbl sym input fuel = (Some tr, suffix)
-              | (Node x f) => exists fuel fuel2 gamma,
-                              parseTableLookup x (peek input) tbl = Some gamma
-                              /\ parseForest tbl gamma input fuel = (Some f, suffix)
-                              /\ parse tbl sym input fuel2 = (Some tr, suffix)
-              end)
-      (P0 := fun subtrees =>
-               forall input gamma prefix suffix,
-                     input = (prefix ++ suffix)%list ->
-                     (@derivesForest g) gamma prefix subtrees ->
-                     exists x fuel, parseTableLookup x (peek input) tbl= Some gamma
-                                    /\ parseForest tbl gamma input fuel = (Some subtrees, suffix)).
+               forall g tok toks x,
+                 (@derivesTree g) x (tok :: toks) tr
+                 -> (@firstSym g) (LA tok) x); intros.
 
-  - intros.
-    inv H0.
-    exists 1.
-    simpl.
-    assert (Utils.beqString s s = true) by admit.
-    rewrite H.
-    trivial.
+  - inv H.
+    constructor.
 
-  - intros.
-    inv H0.
-    eapply IHparseForest with (prefix := prefix) (suffix := suffix) (input := app prefix suffix) in H6.
-    + destruct H6 as [x [fuel [ Hl Hpf]]].
-      exists fuel. exists (S fuel). exists gamma.
-      split.
-      * trivial.
-*)
+  - inv H.
+    apply IHf with (tok := tok) (toks := toks) in H5.
+    eapply FiNT.
+    constructor; eauto.
 
+  - inv H.
+
+  - inv H.
+    destruct prefix.
+    + simpl in *.
+      subst.
+      apply IHf0 in H5.
+      destruct hdRoot.
+      * inv H4.
+      * apply FiGammaTl.
+        -- apply derivesTree_nil_nullable in H4.
+           auto.
+        -- auto.
+    + simpl in *.
+      inv H0.
+      apply IHf in H4.
+      apply FiGammaHd.
+      auto.
+Qed.
+
+Lemma derivesForest_cons_firstProd :
+  forall f g tok toks x gamma,
+    In (x, gamma) (productions g)
+    -> (@derivesForest g) gamma (tok :: toks) f
+    -> (@firstProd g) (LA tok) x gamma.
+Proof.
+  intros.
+  constructor; auto.
+  eapply derivesForest_cons_firstGamma.
+  eauto.
+Qed.
+
+Lemma prefixes_eq :
+  forall (suf pre pre' : list string),
+    app pre suf = app pre' suf
+    -> pre = pre'.
+Proof.
+  induction suf; intros; simpl in *.
+  - repeat rewrite app_nil_r in H.
+    auto.
+  - assert (a :: suf = app [a] suf) by auto.
+    repeat rewrite H0 in H.
+    repeat rewrite app_assoc in H.
+    apply IHsuf in H.
+    apply app_inj_tail in H.
+    destruct H.
+    auto.
+Qed.
+    
 Theorem parse_complete :
   forall (g   : grammar)
          (tbl : parse_table),
@@ -389,7 +515,7 @@ Theorem parse_complete :
            (sym    : symbol)
            (prefix suffix : list string),
       input = (prefix ++ suffix)%list ->
-      derivesMaximalTree g sym prefix suffix tr
+      symDerivesMaximalPrefix g sym prefix suffix tr
       -> exists (fuel : nat),
           parse tbl sym input fuel = (Some tr, suffix).
 Proof.
@@ -403,7 +529,7 @@ Proof.
       (P := fun tr =>
               forall input sym prefix suffix,
                 input = (prefix ++ suffix)%list ->
-                derivesMaximalTree g sym prefix suffix tr
+                symDerivesMaximalPrefix g sym prefix suffix tr
                 -> exists (fuel : nat),
                     parse tbl sym input fuel =
                     (Some tr, suffix))
@@ -429,30 +555,230 @@ Proof.
 
   (* hard case *)
   - intros input sym prefix suffix Hinput HderivesTree.
-    inv HderivesTree.
-    inv H.
+    unfold symDerivesMaximalPrefix in HderivesTree.
+    destruct HderivesTree as [Hder Hmax].
+    inv Hder.
     apply IHparseForest with (prefix := prefix)
                              (suffix := suffix)
                              (input := app prefix suffix)
-      in H6; clear IHparseForest; eauto.
-    destruct H6 as [fuel].
-    
-    + destruct H4 as [fuel].
-      exists (S fuel).
-      simpl.
+      in H4; clear IHparseForest; eauto.
+    destruct H4 as [fuel].
+    exists (S fuel).
+    simpl.
       destruct (parseTableLookup s
                                  (peek (prefix ++ suffix)) tbl)
-        as [gamma' |] eqn:Hlkp.
-      * destruct (parseForest tbl gamma' (prefix ++ suffix)
+      as [gamma' |] eqn:Hlkp.
+    * destruct (parseForest tbl gamma' (prefix ++ suffix) fuel)
+        as (o, suffix') eqn:Hpf.
+      destruct o as [f' |].
+      -- rename s into x.
+         assert (parseTableLookup x
+                                  (peek (prefix ++ suffix))
+                                  tbl =
+                 Some gamma).
+         { (* parseForest gamma and parseForest gamma' both
+            succeed -- we should be able to prove that gamma
+            and gamma' are the same *)
+         apply parseForest_correct with (g := g) in H; auto.
+         destruct H as [pre [Happ Hder]].
+         assert (pre = prefix) by
+             (apply prefixes_eq in Happ; auto).
+         subst.
+         pose proof Htbl as Htbl'.
+         destruct Htbl as [Hmin Hcom].
+         destruct prefix as [| ptok ptoks] eqn:Hpre; auto.
+
+           - (* prefix is nil -- we have to look at the suffix 
+                by decomposing it into prefix' and suffix' *)
+             simpl in *.
+             pose proof Hlkp as Hlkp'.
+             apply lookup_exists in Hlkp.
+             destruct Hlkp as [laMap [Hsf Hlf]].
+             apply parseForest_correct with (g := g) in Hpf;
+               auto.
+             destruct Hpf as [prefix' [Happ' Hder']].
+             unfold ptMinimal in Hmin.
+             pose proof Hsf as Hsf2.
+             destruct prefix' as [| ptok' ptoks'].
+             
+             + (* prefix' is nil *)
+               destruct suffix' as [| stok' stoks'];
+                 subst; simpl in *; auto.
+               
+               * (* prefix' and suffix' are nil -- x is 
+                    nullable, and EOF is in FOLLOW(x) *)
+                 apply Hmin with
+                     (la := EOF)
+                     (gamma := gamma') in Hsf; auto.
+                 destruct Hsf as [Hfi | Hfo].
+                 -- apply eof_fprod in Hfi; auto.
+                    inv Hfi.
+                 -- destruct Hfo as [Hnp Hfp].
+                    inv Hfp.
+                    assert (Hlkf : (@isLookaheadFor g) EOF x gamma).
+                    { unfold isLookaheadFor.
+                      right.
+                      apply derivesForest_nil_nullable in Hder.
+                      split; constructor; auto. }
+                    apply Hcom in Hlkf.
+                    destruct Hlkf as [laMap' [Hsf' Hlf']].
+                    congruence.
+                    
+               * (* prefix' is nil, suffix' is cons -- stok' 
+                    is in FOLLOW(x), but I'm not sure how to
+                    handle the FIRST case *)
+                 apply Hmin with (la := LA stok')
+                                 (gamma := gamma') in Hsf; auto.
+                 destruct Hsf as [Hfi | Hfo].
+                 -- admit.
+                 -- destruct Hfo as [Hnp Hfp].
+                    inv Hfp.
+                    assert (Hlkf : (@isLookaheadFor g) (LA stok') x gamma).
+                    { unfold isLookaheadFor.
+                      right.
+                      apply derivesForest_nil_nullable in Hder.
+                      split; constructor; auto. }
+                    apply Hcom in Hlkf.
+                    destruct Hlkf as [laMap' [Hsf' Hlf']].
+                    congruence.
+                    
+             + (* prefix' is cons -- this violates the
+                  Hmax hypothesis *)
+               apply lookup_tbl_in_grammar
+                 with (g := g) in Hlkp'; auto.
+               assert ((@derivesTree g) (NT x)
+                                          (ptok' :: ptoks')
+                                          (Node x f')).
+               { eapply derivesNT.
+                 { apply Hlkp'. }
+                 { auto. }}
+               eapply Hmax in H; eauto.
+                 simpl in H.
+                 inv H.
+
+           - (* prefix is ptok :: ptoks -- ptok is in 
+                FIRST for (x, gamma) *)
+             eapply derivesForest_cons_firstProd in Hder;
+               eauto.
+             assert ((@isLookaheadFor g) (LA ptok) x gamma) by
+                 (unfold isLookaheadFor; auto).
+             apply Hcom in H.
+             destruct H as [laMap' [Hsf' Hlf']].
+             simpl in *.
+             assert (parseTableLookup x (LA ptok) tbl =
+                     Some gamma).
+             { unfold parseTableLookup.
+               rewrite Hsf'.
+               rewrite Hlf'.
+               auto. }
+             congruence. }
+
+         congruence. (* Made it! *)
+
+      -- (* This case should follow a similar pattern *)
+        apply parseForest_correct with (g := g) in H; auto.
+         destruct H as [pre [Happ Hder]].
+         assert (pre = prefix) by admit.
+         pose proof Hlkp as Hlkp'.
+         apply lookup_exists in Hlkp.
+         destruct Hlkp as [laMap [Hsf Hlf]].
+         pose proof Htbl as Htbl'.
+         unfold isParseTableFor in Htbl.
+         destruct Htbl as [Hmin Hcom].
+         apply parseForest_correct with (g := g) in Hpf; auto.
+         destruct Hpf as [prefix' [Happ' Hder']].
+         destruct prefix as [| ptok ptoks] eqn:Hpre.
+         
+
+             
+           - eapply derivesForest_cons_firstProd in Hder;
+               eauto.
+             assert ((@isLookaheadFor g) (LA ptok) x gamma) by
+                 (unfold isLookaheadFor; auto).
+             apply Hcom in H.
+             destruct H as [laMap' [Hsf' Hlf']].
+             simpl in *.
+             congruence. }
+         congruence.
+
+      -- 
+
+         
+
+           - auto.
+           - 
+         ++ (* prefix and suffix are nil *)
+           apply derives_nil_nullable in Hder.
+           unfold ptMinimal in Hmin.
+           pose proof Hsf as Hsf1.
+           apply Hmin with (gamma := gamma') (la := EOF) in Hsf.
+           destruct Hsf as [Hfp | Hnp].
+           ** apply eof_fprod in Hfp; inv Hfp; trivial.
+           ** (* Now we know that (x, gamma') is nullable
+                 and that EOF is in FOLLOW(x). We should be
+                 able to prove that EOF is a lookahead symbol
+                 for (x, gamma) *)
+             destruct Hnp as [Hnp Hfp].
+             inv Hfp.
+             assert (Hlkf : (@isLookaheadFor g) EOF x gamma).
+             { unfold isLookaheadFor.
+               right; split.
+               { constructor; auto. }
+               { constructor; auto. }}
+             apply Hcom in Hlkf.
+             destruct Hlkf as [laMap' [Hsf' Hlf']].
+             congruence.
+           ** auto.
+         ++ (* prefix is nil, suffix is (stok :: stoks) *)
+           apply derives_nil_nullable in Hder.
+           unfold ptMinimal in Hmin.
+           pose proof Hsf as Hsf1.
+           apply Hmin with (gamma := gamma') (la := LA stok)
+             in Hsf.
+           ** destruct Hsf as [Hfi | Hfo].
+              --- (* stok in FIRST for (x, gamma'). 
+                     This should mean that prefix' isn't empty.
+                     prefix is empty, though -- that should
+                     violate the Hmax hypothesis *)
+                apply firstProd_not_nil with
+                    (tbl := tbl)
+                    (word := prefix')
+                    (f := f') in Hfi; admit.
+              ---admit.
+           ** admit.
+         ++ apply derives_cons_fprod
+              with (x := x) in Hder; auto.
+            assert ((@isLookaheadFor g) (LA ptok)
+                                        x gamma).
+            { unfold isLookaheadFor.
+              left.
+              auto. }
+            unfold ptComplete in Hcom.
+            apply Hcom in H.
+            destruct H as [laMap' [Hsf' Hlf']].
+            congruence.
+                     
+               
+
+
+
+
+
+
+
+
+
+
+
+
+
+      
+    * destruct (parseForest tbl gamma' (prefix ++ suffix)
                               fuel)
           as (o, suffix') eqn:Hpf.
         destruct o as [f' |].
-        -- unfold parseTableLookup in Hlkp.
-           
-      eapply in_grammar_lookup_tbl in Htbl; eauto.
-      rewrite Htbl.
-      rewrite H.
-      trivial.
+      -- admit.
+      -- 
 
   - intros x input gamma prefix suffix Hinput HderivesForest.
     inv HderivesForest.
